src/program_proof/buftxn/specs.v
@@ -1,0 +1,142 @@
+From RecordUpdate Require Import RecordSet.
+Import RecordSetNotations.
+
+From Perennial.Helpers Require Import Transitions.
+From Perennial.program_proof Require Import proof_prelude.
+From Perennial.Helpers Require Import GenHeap.
+From Perennial.goose_lang.lib Require Import struct.
+
+From Goose.github_com.mit_pdos.goose_nfsd Require Import addr buftxn.
+From Perennial.program_proof Require Import txn.specs.
+
+Section heap.
+Context `{!heapG Σ}.
+Context `{!lockG Σ}.
+Context `{!inG Σ (authR (optionUR (exclR boolO)))}.
+
+Implicit Types s : Slice.t.
+Implicit Types (stk:stuckness) (E: coPset).
+
+Definition is_buftxn (buftx : loc) (γT γUnified : gen_heapG addr txnObject Σ) : iProp Σ :=
+  (
+    ∃ (l : loc) mT bufmap (txid : u64) gBits gInodes gBlocks,
+      buftx ↦[BufTxn.S :: "txn"] #l ∗
+      buftx ↦[BufTxn.S :: "bufs"] #bufmap ∗
+      buftx ↦[BufTxn.S :: "Id"] #txid ∗
+      is_txn l gBits gInodes gBlocks ∗
+      unify_heaps gBits gInodes gBlocks γUnified ∗
+      gen_heap_ctx (hG := γT) mT ∗
+      [∗ map] a ↦ v ∈ mT,
+        ∃ v0,
+          mapsto (hG := γUnified) a 1 v0
+  )%I.
+
+Theorem wp_buftxn_Begin l gBits gInodes gBlocks γUnified :
+  {{{ is_txn l gBits gInodes gBlocks ∗
+      unify_heaps gBits gInodes gBlocks γUnified
+  }}}
+    Begin #l
+  {{{ (buftx : loc) γt, RET #buftx;
+      is_buftxn buftx γt γUnified
+  }}}.
+Proof.
+  iIntros (Φ) "(Htxn & Hunified) HΦ".
+Admitted.
+
+Theorem wp_BufTxn__ReadBuf__Block buftx γt γUnified a aa v :
+  {{{
+    is_buftxn buftx γt γUnified ∗
+    ⌜ getField_f Addr.S "Sz" a = #(U64 (block_bytes*8)%nat) ⌝ ∗
+    ⌜ getField_f Addr.S "Blkno" a = #aa.(addrBlock) ⌝ ∗
+    ⌜ getField_f Addr.S "Off" a = #aa.(addrOff) ⌝ ∗
+    mapsto (hG := γt) aa 1 (txnBlock v)
+  }}}
+    BufTxn__ReadBuf #buftx a
+  {{{
+    (buf : Slice.t), RET (slice_val buf);
+    is_slice buf u8T 1%Qp (Block_to_vals v) ∗
+    is_buftxn buftx γt γUnified ∗
+    mapsto (hG := γt) aa 1 (txnBlock v)
+  }}}.
+Proof.
+  iIntros (Φ) "(Htxn & % & % & % & Ha) HΦ".
+  iDestruct "Htxn" as (l mT bufmap txid gBits gInodes gBlocks) "(Hl & Hbufmap & Htxid & Htxn & Hunify & Hγtctx & Hm)".
+  wp_call.
+  wp_loadField.
+Admitted.
+
+Theorem wp_BufTxn__OverWrite__Block buftx γt γUnified a aa v0 v (buf : Slice.t) :
+  {{{
+    is_buftxn buftx γt γUnified ∗
+    ⌜ getField_f Addr.S "Sz" a = #(U64 (block_bytes*8)%nat) ⌝ ∗
+    ⌜ getField_f Addr.S "Blkno" a = #aa.(addrBlock) ⌝ ∗
+    ⌜ getField_f Addr.S "Off" a = #aa.(addrOff) ⌝ ∗
+    mapsto (hG := γt) aa 1 (txnBlock v0) ∗
+    is_slice buf u8T 1%Qp (Block_to_vals v)
+  }}}
+    BufTxn__OverWrite #buftx a (slice_val buf)
+  {{{
+    RET #();
+    is_buftxn buftx γt γUnified ∗
+    mapsto (hG := γt) aa 1 (txnBlock v)
+  }}}.
+Proof.
+  iIntros (Φ) "(Htxn & % & % & % & Ha & Hbuf) HΦ".
+  iDestruct "Htxn" as (l mT bufmap txid gBits gInodes gBlocks) "(Hl & Hbufmap & Htxid & Htxn & Hunify & Hγtctx & Hm)".
+  wp_call.
+  wp_loadField.
+Admitted.
+
+Theorem BufTxn_lift buftx γt γUnified a v :
+  (
+    is_buftxn buftx γt γUnified ∗
+    mapsto (hG := γUnified) a 1 v
+  )
+    ==∗
+  (
+    is_buftxn buftx γt γUnified ∗
+    mapsto (hG := γt) a 1 v
+  ).
+Proof.
+  iIntros "[Htxn Ha]".
+  iDestruct "Htxn" as (l mT bufmap txid gBits gInodes gBlocks) "(Hl & Hbufmap & Htxid & Htxn & Hunify & Hγtctx & Hm)".
+  iAssert (⌜ mT !! a = None ⌝)%I as %Hnone.
+  {
+    destruct (mT !! a) eqn:He; eauto.
+    iDestruct (big_sepM_lookup with "Hm") as (v2) "Ha2"; eauto.
+    iDestruct (mapsto_valid_2 with "Ha Ha2") as %Ha.
+    exfalso. eauto.
+  }
+
+  iMod ((gen_heap_alloc _ _ v) with "Hγtctx") as "[Hγtctx Haa]"; eauto.
+  iModIntro.
+  iSplitR "Haa"; [|iFrame].
+
+  iExists _, _, _, _, _, _, _.
+  iFrame.
+  iApply (big_sepM_insert); eauto.
+  iFrame.
+  iExists _; iFrame.
+Qed.
+
+Theorem wp_BufTxn__CommitWait buftx γt γUnified mods :
+  {{{
+    is_buftxn buftx γt γUnified ∗
+    [∗ map] a ↦ v ∈ mods, mapsto (hG := γt) a 1 v
+  }}}
+    BufTxn__CommitWait #buftx #true
+  {{{
+    RET #();
+    [∗ map] a ↦ v ∈ mods, mapsto (hG := γUnified) a 1 v
+  }}}.
+Proof.
+  iIntros (Φ) "(Htxn & Hmods) HΦ".
+  iDestruct "Htxn" as (l mT bufmap txid gBits gInodes gBlocks) "(Hl & Hbufmap & Htxid & Htxn & Hunify & Hγtctx & Hm)".
+
+  wp_call.
+  wp_apply util_proof.wp_DPrintf.
+  wp_loadField.
+  wp_loadField.
+Admitted.
+
+End heap.
